demo/fib/Fib6.v
@@ -15,14 +15,34 @@ Set Implicit Arguments.
 
 
 
+Definition f_fib_ru (oh0: owned_heap) (m0: mem) (vs0: list val):
+  itree (E owned_heap) (owned_heap * (mem * val)) :=
+  `n: nat <- (unwrapN (parse_arg oh0 m0 vs0)) ;;
+    match n with
+    | O => Ret (oh0, (m0, (Vint Int.zero)))
+    | S O => Ret (oh0, (m0, (Vint Int.one)))
+    | S (S m) =>
+      let vs0 := [Vint (of_nat m)] in
+
+      '(oh1, (m1, y1)) <- trigger (ICall _fib_ru oh0 m0 vs0) ;;
+
+      let vs1 := [Vint (of_nat (S m))] in
+
+      '(oh2, (m2, y2)) <- trigger (ICall _fib_ru oh1 m1 vs1) ;;
+
+      Ret (oh2, (m2, Vint (of_nat (fib_nat n))))
+    end
+.
+
 Definition f_fib (oh0: owned_heap) (m0: mem) (vs0: list val):
   itree (E owned_heap) (owned_heap * (mem * val)) :=
   assume (precond oh0 m0 vs0) ;;
+  tau;;
   ohmv <- trigger (EChoose { ohmv: (owned_heap * (mem * val)) | postcond oh0 m0 vs0 ohmv }) ;;
   Ret (proj1_sig ohmv)
 .
 
 Definition prog: program owned_heap :=
-  (Maps.add _fib f_fib Maps.empty).
+  (Maps.add _fib_ru f_fib_ru (Maps.add _fib f_fib Maps.empty)).
 
 Definition module: Mod.t := module (Fib0.module) prog "fib"%string initial_owned_heap.
